

STAT 1150 Formula Sheet

$$1. s = \sqrt{\frac{\sum_{i=1}^n (x_i - \bar{x})^2}{n-1}}$$

$$2. z = \frac{\hat{p} - p}{\sqrt{\frac{p(1-p)}{n}}}$$

$$3. n = \left(\frac{z^* \sigma}{m}\right)^2$$

$$4. \hat{p} \pm z^* \sqrt{\frac{\hat{p}(1-\hat{p})}{n}}$$

$$5. n = \left(\frac{z^*}{m}\right)^2 p^*(1-p^*)$$

$$6. z = \frac{\hat{p} - p_0}{\sqrt{\frac{p_0(1-p_0)}{n}}}$$

$$7. \bar{x}_d \pm t^* \frac{s_d}{\sqrt{n}}$$

$$8. t = \frac{\bar{x}_d}{s_d/\sqrt{n}}$$

$$9. \bar{x}_1 - \bar{x}_2 \pm t^* \sqrt{s_p^2 \left(\frac{1}{n_1} + \frac{1}{n_2}\right)}$$

$$10. t = \frac{\bar{x}_1 - \bar{x}_2}{\sqrt{s_p^2 \left(\frac{1}{n_1} + \frac{1}{n_2}\right)}}$$

$$\text{where } s_p^2 = \frac{(n_1 - 1)s_1^2 + (n_2 - 1)s_2^2}{n_1 + n_2 - 2}$$

$$11. \bar{x}_1 - \bar{x}_2 \pm t^* \sqrt{\frac{s_1^2}{n_1} + \frac{s_2^2}{n_2}}$$

$$12. t = \frac{\bar{x}_1 - \bar{x}_2}{\sqrt{\frac{s_1^2}{n_1} + \frac{s_2^2}{n_2}}}$$

$$13. \ r = \frac{1}{(n-1)s_x s_y} \sum_{i=1}^n (x_i - \bar{x})(y_i - \bar{y})$$

$$14. \ b_1 = r \frac{s_y}{s_x} = \frac{\sum_{i=1}^n (x_i - \bar{x})(y_i - \bar{y})}{\sum_{i=1}^n (x_i - \bar{x})^2}$$

$$15 \ b_0 = \bar{y} - b_1 \bar{x}$$

$$16. \ s_e = \sqrt{\frac{\sum_{i=1}^n (y_i - \hat{y}_i)^2}{n-2}}$$

$$17. \ \hat{y} \pm t^* SE_{\hat{\mu}}$$

$$\text{where} \quad SE_{\hat{\mu}} = s_e \sqrt{\frac{1}{n} + \frac{(x^* - \bar{x})^2}{\sum_{i=1}^n (x_i - \bar{x})^2}}$$

$$18. \ b_1 \pm t^* SE_{b_1}$$

$$19. \ t = \frac{b_1}{SE_{b_1}}$$

$$\text{where} \quad SE_{b_1} = \frac{s_e}{\sqrt{\sum_{i=1}^n (x_i - \bar{x})^2}}$$